src/Init/Data/Iterators/Lemmas/Consumers/Monadic/Loop.lean
@@ -15,28 +15,26 @@ namespace Std.Iterators
 
 theorem IterM.DefaultConsumers.forIn'_eq_match_step {α β : Type w} {m : Type w → Type w'}
     [Iterator α m β]
-    {n : Type w → Type w''} [Monad n]
-    {lift : ∀ γ, m γ → n γ} {γ : Type w}
+    {n : Type x → Type x'} [Monad n]
+    {lift : ∀ γ δ, (γ → n δ) → m γ → n δ} {γ : Type x}
     {plausible_forInStep : β → γ → ForInStep γ → Prop}
     {wf : IteratorLoop.WellFounded α m plausible_forInStep}
     {it : IterM (α := α) m β} {init : γ}
-    {P hP}
-    {f : (b : β) → P b → (c : γ) → n (Subtype (plausible_forInStep b c))} :
-    IterM.DefaultConsumers.forIn' lift γ plausible_forInStep wf it init P hP f = (do
-      match ← lift _ it.step with
-      | .yield it' out h =>
-        match ← f out (hP _ <| .direct ⟨_, h⟩) init with
-        | ⟨.yield c, _⟩ =>
-          IterM.DefaultConsumers.forIn' lift _ plausible_forInStep wf it' c P
-            (fun _ h' => hP _ <| .indirect ⟨_, rfl, h⟩ h') f
-        | ⟨.done c, _⟩ => return c
-      | .skip it' h =>
-        IterM.DefaultConsumers.forIn' lift _ plausible_forInStep wf it' init P
-          (fun _ h' => hP _ <| .indirect ⟨_, rfl, h⟩ h') f
-      | .done _ => return init) := by
+    {P hP} {f : (b : β) → P b → (c : γ) → n (Subtype (plausible_forInStep b c))} :
+    IterM.DefaultConsumers.forIn' lift γ plausible_forInStep wf it init P hP f =
+      (lift _ _ · it.step) (fun
+          | .yield it' out h => do
+            match ← f out (hP _ <| .direct ⟨_, h⟩) init with
+            | ⟨.yield c, _⟩ =>
+              IterM.DefaultConsumers.forIn' lift _ plausible_forInStep wf it' c P
+                (fun _ h' => hP _ <| .indirect ⟨_, rfl, h⟩ h') f
+            | ⟨.done c, _⟩ => return c
+          | .skip it' h =>
+            IterM.DefaultConsumers.forIn' lift _ plausible_forInStep wf it' init P
+              (fun _ h' => hP _ <| .indirect ⟨_, rfl, h⟩ h') f
+          | .done _ => return init) := by
   rw [forIn']
-  apply bind_congr
-  intro step
+  congr; ext step
   cases step using PlausibleIterStep.casesOn <;> rfl
 
 theorem IterM.forIn'_eq {α β : Type w} {m : Type w → Type w'} [Iterator α m β] [Finite α m]
@@ -44,7 +42,8 @@ theorem IterM.forIn'_eq {α β : Type w} {m : Type w → Type w'} [Iterator α m
     [MonadLiftT m n] {γ : Type w} {it : IterM (α := α) m β} {init : γ}
     {f : (b : β) → it.IsPlausibleIndirectOutput b → γ → n (ForInStep γ)} :
     letI : ForIn' n (IterM (α := α) m β) β _ := IterM.instForIn'
-    ForIn'.forIn' it init f = IterM.DefaultConsumers.forIn' (fun _ => monadLift) γ (fun _ _ _ => True)
+    ForIn'.forIn' it init f = IterM.DefaultConsumers.forIn' (n := n)
+        (fun _ _ f x => monadLift x >>= f) γ (fun _ _ _ => True)
         IteratorLoop.wellFounded_of_finite it init _ (fun _ => id) ((⟨·, .intro⟩) <$> f · · ·) := by
   cases hl.lawful; rfl
 
@@ -52,14 +51,15 @@ theorem IterM.forIn_eq {α β : Type w} {m : Type w → Type w'} [Iterator α m 
     {n : Type w → Type w''} [Monad n] [IteratorLoop α m n] [hl : LawfulIteratorLoop α m n]
     [MonadLiftT m n] {γ : Type w} {it : IterM (α := α) m β} {init : γ}
     {f : β → γ → n (ForInStep γ)} :
-    ForIn.forIn it init f = IterM.DefaultConsumers.forIn' (fun _ => monadLift) γ (fun _ _ _ => True)
+    ForIn.forIn it init f = IterM.DefaultConsumers.forIn' (n := n)
+        (fun _ _ f x => monadLift x >>= f) γ (fun _ _ _ => True)
         IteratorLoop.wellFounded_of_finite it init _ (fun _ => id) (fun out _ acc => (⟨·, .intro⟩) <$> f out acc) := by
   cases hl.lawful; rfl
 
 theorem IterM.DefaultConsumers.forIn'_eq_forIn' {m : Type w → Type w'} {α : Type w} {β : Type w}
     [Iterator α m β]
-    {n : Type w → Type w''} [Monad n]
-    {lift : ∀ γ, m γ → n γ} {γ : Type w}
+    {n : Type x → Type x'} [Monad n]
+    {liftBind : ∀ γ δ, (γ → n δ) → m γ → n δ} {γ : Type x}
     {Pl : β → γ → ForInStep γ → Prop}
     {wf : IteratorLoop.WellFounded α m Pl}
     {it : IterM (α := α) m β} {init : γ}
@@ -68,11 +68,10 @@ theorem IterM.DefaultConsumers.forIn'_eq_forIn' {m : Type w → Type w'} {α : T
     {f : (b : β) → P b → (c : γ) → n (Subtype (Pl b c))}
     {g : (b : β) → Q b → (c : γ) → n (Subtype (Pl b c))}
     (hfg : ∀ b c, (hPb : P b) → (hQb : Q b) → f b hPb c = g b hQb c) :
-    IterM.DefaultConsumers.forIn' lift γ Pl wf it init P hP f =
-      IterM.DefaultConsumers.forIn' lift γ Pl wf it init Q hQ g := by
+    IterM.DefaultConsumers.forIn' liftBind γ Pl wf it init P hP f =
+      IterM.DefaultConsumers.forIn' liftBind γ Pl wf it init Q hQ g := by
   rw [forIn', forIn']
-  apply bind_congr
-  intro step
+  congr; ext step
   split
   · congr
     · apply hfg
@@ -138,8 +137,7 @@ theorem IterM.forIn_eq_match_step {α β : Type w} {m : Type w → Type w'} [Ite
       | .skip it' _ => ForIn.forIn it' init f
       | .done _ => return init) := by
   simp only [forIn]
-  rw [forIn'_eq_match_step]
-  rfl
+  exact forIn'_eq_match_step
 
 theorem IterM.forM_eq_forIn {α β : Type w} {m : Type w → Type w'} [Iterator α m β]
     [Finite α m] {n : Type w → Type w''} [Monad n] [LawfulMonad n]
